MirrorCharge!/src/MirrorCharge/Imp/RTacSubst.v
@@ -1,0 +1,100 @@
+Require Import MirrorCore.Lambda.Expr.
+Require Import MirrorCore.RTac.RTac.
+Require MirrorCore.syms.SymEnv.
+Require MirrorCore.syms.SymSum.
+Require Import MirrorCore.Lambda.ExprUnify_simul.
+Require Import MirrorCharge.ILogicFunc.
+Require Import MirrorCharge.OrderedCanceller.
+Require Import MirrorCharge.BILNormalize.
+Require Import MirrorCharge.SynSepLog.
+Require Import MirrorCharge.SepLogFold.
+Require Import MirrorCharge.Imp.Syntax.
+Require Import MirrorCharge.Tauto.
+Require Import MirrorCharge.Imp.ImpTac.
+
+Set Implicit Arguments.
+Set Strict Implicit.
+
+Local Existing Instance SS.
+Local Existing Instance SU.
+Local Existing Instance RSym_ilfunc.
+Local Existing Instance RS.
+Local Existing Instance Expr_expr.
+
+Record Eq_spec : Type :=
+{ as_eq : expr typ func -> option (typ * expr typ func * expr typ func) }.
+
+Section subst.
+  Variable eq_spec : Eq_spec.
+  Variable ilspec : ILogicSpec typ func.
+
+  Require Import ExtLib.Core.RelDec.
+
+  Fixpoint find_in_list (n : nat) (ls : list (nat * expr typ func))
+  : option (expr typ func) :=
+    match ls with
+      | nil => None
+      | cons (n',e) ls =>
+        if n ?[eq] n' then Some e else find_in_list n ls
+    end.
+
+  Section the_subst.
+    Variable ss : list (nat * expr typ func).
+
+    Fixpoint subst  (u : nat) (e : expr typ func)
+    : expr typ func :=
+      match e with
+        | ExprCore.Var v =>
+          match Nat.lt_rem v u with
+            | None => Var v
+            | Some k =>
+              match find_in_list k ss with
+                | None => e
+                | Some e' => lift 0 u e'
+              end
+          end
+        | ExprCore.UVar _
+        | ExprCore.Inj _ => e
+        | ExprCore.App l r => ExprCore.App (subst u l) (subst u r)
+        | ExprCore.Abs t l => ExprCore.Abs t (subst (S u) l)
+      end.
+  End the_subst.
+
+  Fixpoint gather (e : expr typ func)
+  : expr typ func * list (nat * expr typ func) :=
+    match eq_spec.(as_eq) e with
+      | Some (t,l,r) =>
+        match l with
+          | ExprCore.Var v => (Syntax.ltrue tyProp, (v,r) :: nil)
+          | _ =>
+            match r with
+              | ExprCore.Var v => (Syntax.ltrue tyProp, (v,l) :: nil)
+              | _ => (e,nil)
+            end
+        end
+      | None =>
+        match e with
+          | App (App bop l) r =>
+            match ilspec.(as_logic) bop with
+              | Some LAnd =>
+                let (l',eqsl) := gather l in
+                let (r',eqsr) := gather r in
+                (App (App bop l') r', eqsl ++ eqsr)
+              | Some LImpl =>
+                let (l',eqsl) := gather l in
+                (App (App bop l) (subst eqsl 0 r), nil)
+              | Some LEntails =>
+                let (l',eqsl) := gather l in
+                (App (App bop l) (subst eqsl 0 r), nil)
+              | _ => (e,nil)
+            end
+          | _ => (e,nil)
+        end
+    end.
+
+  Definition subst_tac : imp_tac :=
+    fun tus tvs _ _ ctx sub g =>
+      let (g',_) := gather g in
+      More_ sub (GGoal g').
+
+End subst.
