MirrorCharge!/src/MirrorCharge/Imp/RTacTauto.v
@@ -1,0 +1,67 @@
+Require Import MirrorCore.Lambda.Expr.
+Require Import MirrorCore.RTac.RTac.
+Require MirrorCore.syms.SymEnv.
+Require MirrorCore.syms.SymSum.
+Require Import MirrorCore.Lambda.ExprUnify_simul.
+Require Import MirrorCharge.ILogicFunc.
+Require Import MirrorCharge.OrderedCanceller.
+Require Import MirrorCharge.BILNormalize.
+Require Import MirrorCharge.SynSepLog.
+Require Import MirrorCharge.SepLogFold.
+Require Import MirrorCharge.Imp.Syntax.
+Require Import MirrorCharge.Tauto.
+Require Import MirrorCharge.Imp.ImpTac.
+
+Set Implicit Arguments.
+Set Strict Implicit.
+
+Local Existing Instance SS.
+Local Existing Instance SU.
+Local Existing Instance RSym_ilfunc.
+Local Existing Instance RS.
+Local Existing Instance Expr_expr.
+
+Definition ILogicSpec_sym : ILogicSpec typ func :=
+{| as_logic := fun e =>
+                match e with
+                  | Inj (inr (ILogicFunc.ilf_true _)) => Some LTrue
+                  | Inj (inr (ILogicFunc.ilf_false _)) => Some LFalse
+                  | Inj (inr (ILogicFunc.ilf_and _)) => Some LAnd
+                  | Inj (inr (ILogicFunc.ilf_or _)) => Some LOr
+                  | Inj (inr (ILogicFunc.ilf_impl _)) => Some LImpl
+                  | Inj (inr (ILogicFunc.ilf_entails _)) => Some LEntails
+                  | _ => None
+                end
+ |}.
+
+Definition EmbedSpec_sym : EmbedSpec typ func :=
+{| is_embed := fun e =>
+                match e with
+                  | Inj (inr (ILogicFunc.ilf_embed _ t)) => Some t
+                  | _ => None
+                end
+ |}.
+
+Definition floor (e : expr typ func) (from to : typ) : option (expr typ func) :=
+  None.
+
+Axiom todo : forall {T : Type}, T.
+
+Definition tauto_tac : imp_tac :=
+  fun tus tvs _ _ ctx sub e =>
+    match e with
+      | App (App (Inj (inr (ILogicFunc.ilf_entails t))) P) Q =>
+        match learn ILogicSpec_sym P nil with
+          | None => Solved sub
+          | Some ps =>
+            match Tauto.tauto_simplify tyProp ILogicSpec_sym EmbedSpec_sym floor _ ps Q t with
+              | None => Solved sub
+              | Some Q' =>
+                More_ sub (GGoal (App (App (Inj (inr (ILogicFunc.ilf_entails t))) P) Q'))
+            end
+        end
+      | _ => Fail
+    end.
+
+Theorem tauto_tac_sound : rtac_sound tauto_tac.
+Admitted.
